no message

execution/examples/Dexter2CPMM.v
@@ -1,4 +1,4 @@
-From Coq Require Import ZArith.
+From Coq Require Import ZArith Lia.
 From Coq Require Import Morphisms.
 Require Import Monads.
 Require Import Extras.
@@ -136,7 +136,8 @@ Record State :=
     manager : Address;
     tokenAddress : Address;
     tokenId : token_id;
-    lqtAddress : option Address
+    lqtAddress : Address;
+    nullAddress : Address
   }.
 
 Record Setup :=
@@ -144,7 +145,8 @@ Record Setup :=
     lqtTotal_ : N;
     manager_ : Address;
     tokenAddress_ : Address;
-    tokenId_ : token_id
+    tokenId_ : token_id;
+    nullAddress_ : Address
   }.
 
 MetaCoq Run (make_setters State).
@@ -171,11 +173,25 @@ Definition isNone {A : Type} (a : option A) := match a with | Some _ => false | 
 Definition isSome {A : Type} (a : option A) := negb (isNone a).
 Definition returnIf (cond : bool) := if cond then None else Some tt.
 Definition is_a_nat (n : Z) : bool := Z.leb 0 n.
-Definition ceildiv (n m : N) : N := if N.modulo n m =? 0 then n / m else (n / m) + 1.
+Definition div (n m : N) : option N := do _ <- returnIf (m =? 0) ; Some (n / m).
+Definition ceildiv (n m : N) : option N :=
+  if N.modulo n m =? 0
+  then div n m
+  else do result <- div n m ; Some (result + 1).
+Definition ceildiv_ (n m : N) : N :=
+  if N.modulo n m =? 0
+  then n / m
+  else (n / m) + 1.
+Opaque ceildiv.
+Opaque ceildiv_.
+Opaque div.
+
+(* Place holder for tezos set delegate operation *)
+Definition set_delegate_call (addr : option Address) : list ActionBody := [].
 
 Definition mint_or_burn (state : State) (target : Address) (quantitiy : Z) : option ActionBody :=
-    do lqtAddress_ <- state.(lqtAddress) ; (* error lqtAddress not set *)
-    Some (act_call lqtAddress_ 0%Z
+    do _ <- returnIf (address_eqb state.(lqtAddress) state.(nullAddress)) ; (* error lqtAddress not set *)
+    Some (act_call state.(lqtAddress) 0%Z
         (serialize (Dexter2FA12.msg_mint_or_burn
         (Dexter2FA12.build_mintOrBurn_param quantitiy target)))).
 
@@ -198,8 +214,8 @@ Definition add_liquidity (chain : Chain) (ctx : ContractCallContext)
                          : result :=
   do _ <- returnIf state.(selfIsUpdatingTokenPool) ; (* error_SELF_IS_UPDATING_TOKEN_POOL_MUST_BE_FALSE *)
   do _ <- returnIf (param.(add_deadline) <=? chain.(current_slot))%nat ; (* error_THE_CURRENT_TIME_MUST_BE_LESS_THAN_THE_DEADLINE *)
-  let lqt_minted := (Z.to_N ctx.(ctx_amount)) * state.(lqtTotal)  / state.(xtzPool) in
-  let tokens_deposited := ceildiv ((Z.to_N ctx.(ctx_amount)) * state.(tokenPool)) state.(xtzPool) in
+  do lqt_minted <- div ((Z.to_N ctx.(ctx_amount)) * state.(lqtTotal)) state.(xtzPool) ; (* error_DIV_by_0 *)
+  do tokens_deposited <- ceildiv ((Z.to_N ctx.(ctx_amount)) * state.(tokenPool)) state.(xtzPool) ; (* error_DIV_by_0 *)
   do _ <- returnIf (param.(maxTokensDeposited) <? tokens_deposited) ; (* error_MAX_TOKENS_DEPOSITED_MUST_BE_GREATER_THAN_OR_EQUAL_TO_TOKENS_DEPOSITED *)
   do _ <- returnIf (lqt_minted <? param.(minLqtMinted)) ; (* error_LQT_MINTED_MUST_BE_GREATER_THAN_MIN_LQT_MINTED *)
   let new_state := state<| lqtTotal := state.(lqtTotal) + lqt_minted |>
@@ -215,8 +231,8 @@ Definition remove_liquidity (chain : Chain) (ctx : ContractCallContext)
   do _ <- returnIf state.(selfIsUpdatingTokenPool) ; (* error_SELF_IS_UPDATING_TOKEN_POOL_MUST_BE_FALSE *)
   do _ <- returnIf (param.(remove_deadline) <=? chain.(current_slot))%nat ; (* error_THE_CURRENT_TIME_MUST_BE_LESS_THAN_THE_DEADLINE *)
   do _ <- returnIf (0 <? ctx.(ctx_amount))%Z ; (* error_AMOUNT_MUST_BE_ZERO *)
-  let xtz_withdrawn := ((param.(lqtBurned) * state.(xtzPool)) / state.(lqtTotal)) in
-  let tokens_withdrawn := param.(lqtBurned) * state.(tokenPool) /  state.(lqtTotal) in
+  do xtz_withdrawn <-  div (param.(lqtBurned) * state.(xtzPool)) state.(lqtTotal) ; (* error_DIV_by_0 *)
+  do tokens_withdrawn <- div (param.(lqtBurned) * state.(tokenPool)) state.(lqtTotal) ; (* error_DIV_by_0 *)
   do _ <- returnIf (xtz_withdrawn <? param.(minXtzWithdrawn)) ; (* error_THE_AMOUNT_OF_XTZ_WITHDRAWN_MUST_BE_GREATER_THAN_OR_EQUAL_TO_MIN_XTZ_WITHDRAWN *)
   do _ <- returnIf (tokens_withdrawn <? param.(minTokensWithdrawn)) ; (* error_THE_AMOUNT_OF_TOKENS_WITHDRAWN_MUST_BE_GREATER_THAN_OR_EQUAL_TO_MIN_TOKENS_WITHDRAWN *)
   do _ <- returnIf (state.(lqtTotal) <? param.(lqtBurned)) ; (* error_CANNOT_BURN_MORE_THAN_THE_TOTAL_AMOUNT_OF_LQT *)
@@ -234,9 +250,9 @@ Definition xtz_to_token (chain : Chain) (ctx : ContractCallContext)
                         : result :=
   do _ <- returnIf state.(selfIsUpdatingTokenPool) ; (* error_SELF_IS_UPDATING_TOKEN_POOL_MUST_BE_FALSE *)
   do _ <- returnIf (param.(xtt_deadline) <=? chain.(current_slot))%nat ; (* error_THE_CURRENT_TIME_MUST_BE_LESS_THAN_THE_DEADLINE *)
-  let tokens_bought :=
-    ((Z.to_N ctx.(ctx_amount)) * 997 * state.(tokenPool)) /
-      (state.(xtzPool) * 1000 + ((Z.to_N ctx.(ctx_amount)) * 997)) in
+  do tokens_bought <- div
+    ((Z.to_N ctx.(ctx_amount)) * 997 * state.(tokenPool))
+      (state.(xtzPool) * 1000 + ((Z.to_N ctx.(ctx_amount)) * 997)) ; (* error_DIV_by_0 *)
   do _ <- returnIf (tokens_bought <? param.(minTokensBought)) ; (* error_TOKENS_BOUGHT_MUST_BE_GREATER_THAN_OR_EQUAL_TO_MIN_TOKENS_BOUGHT *)
   do _ <- returnIf (state.(tokenPool) <? tokens_bought) ; (* error_TOKEN_POOL_MINUS_TOKENS_BOUGHT_IS_NEGATIVE *)
   let new_state := state<| xtzPool := state.(xtzPool) + (Z.to_N ctx.(ctx_amount)) |>
@@ -250,9 +266,9 @@ Definition token_to_xtz (chain : Chain) (ctx : ContractCallContext)
   do _ <- returnIf state.(selfIsUpdatingTokenPool) ; (* error_SELF_IS_UPDATING_TOKEN_POOL_MUST_BE_FALSE *)
   do _ <- returnIf (param.(ttx_deadline) <=? chain.(current_slot))%nat ; (* error_THE_CURRENT_TIME_MUST_BE_LESS_THAN_THE_DEADLINE *)
   do _ <- returnIf (0 <? ctx.(ctx_amount))%Z ; (* error_AMOUNT_MUST_BE_ZERO *)
-  let xtz_bought :=
-    (((param.(tokensSold) * 997 * state.(xtzPool)) /
-      (state.(tokenPool) * 1000 + (param.(tokensSold) * 997)))) in
+  do xtz_bought <- div
+    (param.(tokensSold) * 997 * state.(xtzPool))
+      (state.(tokenPool) * 1000 + (param.(tokensSold) * 997)) ; (* error_DIV_by_0 *)
   do _ <- returnIf (xtz_bought <? param.(minXtzBought)) ; (* error_XTZ_BOUGHT_MUST_BE_GREATER_THAN_OR_EQUAL_TO_MIN_XTZ_BOUGHT *)
   let op_token := token_transfer state ctx.(ctx_from) ctx.(ctx_contract_address) param.(tokensSold) in
   do op_tez <- xtz_transfer param.(xtz_to) (Z.of_N xtz_bought) ;
@@ -273,7 +289,7 @@ Definition set_baker (chain : Chain) (ctx : ContractCallContext)
   do _ <- returnIf (0 <? ctx.(ctx_amount))%Z ; (* error_AMOUNT_MUST_BE_ZERO *)
   do _ <- returnIf (negb (address_eqb ctx.(ctx_from) state.(manager))) ; (* error_ONLY_MANAGER_CAN_SET_BAKER *)
   do _ <- returnIf (state.(freezeBaker)) ; (* error_BAKER_PERMANENTLY_FROZEN *)
-    Some (state<| freezeBaker := param.(freezeBaker_) |>, []).
+    Some (state<| freezeBaker := param.(freezeBaker_) |>, set_delegate_call param.(baker)).
 
 Definition set_manager (chain : Chain) (ctx : ContractCallContext)
                        (state : State) (new_manager : Address)
@@ -289,8 +305,8 @@ Definition set_lqt_address (chain : Chain) (ctx : ContractCallContext)
   do _ <- returnIf state.(selfIsUpdatingTokenPool) ; (* error_SELF_IS_UPDATING_TOKEN_POOL_MUST_BE_FALSE *)
   do _ <- returnIf (0 <? ctx.(ctx_amount))%Z ; (* error_AMOUNT_MUST_BE_ZERO *)
   do _ <- returnIf (negb (address_eqb ctx.(ctx_from) state.(manager))) ; (* error_ONLY_MANAGER_CAN_SET_LQT_ADRESS *)
-  do _ <- returnIf (isSome state.(lqtAddress)) ; (* error_LQT_ADDRESS_ALREADY_SET *)
-    Some (state<| lqtAddress := Some new_lqt_address |>, []).
+  do _ <- returnIf (negb (address_eqb state.(lqtAddress) state.(nullAddress))) ; (* error_LQT_ADDRESS_ALREADY_SET *)
+    Some (state<| lqtAddress := new_lqt_address |>, []).
 
 Definition update_token_pool (chain : Chain) (ctx : ContractCallContext)
                              (state : State) : result :=
@@ -325,9 +341,9 @@ Definition token_to_token (chain : Chain) (ctx : ContractCallContext)
   do _ <- returnIf state.(selfIsUpdatingTokenPool) ; (* error_SELF_IS_UPDATING_TOKEN_POOL_MUST_BE_FALSE *)
   do _ <- returnIf (0 <? ctx.(ctx_amount))%Z ; (* error_AMOUNT_MUST_BE_ZERO *)
   do _ <- returnIf (param.(ttt_deadline) <=? chain.(current_slot))%nat ; (* error_THE_CURRENT_TIME_MUST_BE_LESS_THAN_THE_DEADLINE *)
-  let xtz_bought :=
-    (((param.(tokensSold_) * 997 * state.(xtzPool)) / 
-      (state.(tokenPool) * 1000 + (param.(tokensSold_) * 997)))) in
+  do xtz_bought <- div
+    (param.(tokensSold_) * 997 * state.(xtzPool))
+      (state.(tokenPool) * 1000 + (param.(tokensSold_) * 997)) ; (* error_DIV_by_0 *)
   let new_state := state<| tokenPool := state.(tokenPool) + param.(tokensSold_) |>
                         <| xtzPool := state.(xtzPool) - xtz_bought |> in
   let op1 := token_transfer state ctx.(ctx_from) ctx.(ctx_contract_address) param.(tokensSold_) in
@@ -386,12 +402,702 @@ Definition init (chain : Chain)
     manager := setup.(manager_);
     tokenAddress := setup.(tokenAddress_);
     tokenId := setup.(tokenId_);
-    lqtAddress := None
+    lqtAddress := setup.(nullAddress_);
+    nullAddress := setup.(nullAddress_)
   |}.
 
 Definition contract : Contract Setup Msg State :=
   build_contract init receive.
 
 Section Theories.
+
+Ltac receive_simpl_step :=
+  match goal with
+  | H : Blockchain.receive _ _ _ _ _ = Some (_, _) |- _ =>
+      unfold Blockchain.receive in H; cbn in H
+  | H : receive _ _ _ _ = Some (_, _) |- _ =>
+      unfold receive in H;
+      cbn in H
+  | |- receive _ _ _ _ = _ =>
+      unfold receive; cbn
+  | H : Some _ = Some _ |- _ =>
+      inversion_clear H
+  | H : Some _ = None |- _ =>
+      inversion H
+  | H : None = Some _ |- _ =>
+      inversion H
+  | H : returnIf _ = None |- _ =>
+    let G := fresh "G" in
+      unfold returnIf in H;
+      destruct_match eqn:G in H; try congruence;
+      clear H;
+      rename G into H
+  | H : returnIf _ = Some ?u |- _ =>
+    let G := fresh "G" in
+      unfold returnIf in H;
+      destruct_match eqn:G in H; try congruence;
+      clear H u;
+      rename G into H
+  | H : option_map (fun s : State => (s, _)) match ?m with | Some _ => _ | None => None end = Some _ |- _ =>
+    let a := fresh "H" in
+    destruct m eqn:a in H; try setoid_rewrite a; cbn in *; try congruence
+  | H : match ?m with | Some _ => _ | None => None end = Some _ |- _ =>
+    let a := fresh "H" in
+    destruct m eqn:a in H; try setoid_rewrite a; cbn in *; try congruence
+  | H : option_map (fun s : State => (s, _)) (if ?m then ?a else ?b) = Some _ |- _ =>
+    match a with
+    | None =>
+      let a := fresh "H" in
+      destruct m eqn:a in H; try setoid_rewrite a; cbn in *; try congruence
+    | _ => match b with
+           | None =>
+             let a := fresh "H" in
+             destruct m eqn:a in H; try setoid_rewrite a; cbn in *; try congruence
+           | _ => idtac
+    end end
+  | H : (if ?m then ?a else ?b) = Some _ |- _ =>
+    match a with
+    | None =>
+      let a := fresh "H" in
+      destruct m eqn:a in H; try setoid_rewrite a; cbn in *; try congruence
+    | _ => match b with
+           | None =>
+             let a := fresh "H" in
+             destruct m eqn:a in H; try setoid_rewrite a; cbn in *; try congruence
+           | _ => idtac
+    end end
+  end.
+
+Tactic Notation "receive_simpl" := repeat receive_simpl_step.
+
+Transparent div.
+Transparent ceildiv.
+Transparent ceildiv_.
+Lemma div_eq : forall n m p,
+  div n m = Some p ->
+  n / m = p /\ m <> 0.
+Proof.
+  intros * div_some.
+  unfold div in div_some.
+  cbn in div_some.
+  destruct_match eqn:m_not_zero in div_some;
+    try congruence.
+  receive_simpl.
+  now apply N.eqb_neq in m_not_zero.
+Qed.
+
+Lemma div_zero : forall n m,
+  div n m = None ->
+  m = 0.
+Proof.
+  intros * div_some.
+  cbn in div_some.
+  destruct_match eqn:m_zero in div_some;
+    try congruence.
+  receive_simpl.
+  now apply N.eqb_eq in m_zero.
+Qed.
+Opaque div.
+
+Lemma ceildiv_eq : forall n m p,
+  ceildiv n m = Some p ->
+  ceildiv_ n m = p /\ m <> 0.
+Proof.
+  intros * ceildiv_some.
+  unfold ceildiv_.
+  unfold ceildiv in ceildiv_some.
+  destruct_match eqn:modulo_zero.
+  - now apply div_eq in ceildiv_some.
+  - cbn in ceildiv_some.
+    destruct_match eqn:div_some in ceildiv_some;
+      try congruence.
+    apply div_eq in div_some.
+    now inversion_clear ceildiv_some.
+Qed.
+
+Lemma ceildiv_zero : forall n m,
+  ceildiv n m = None ->
+  m = 0.
+Proof.
+  intros * ceildiv_some.
+  unfold ceildiv in ceildiv_some.
+  destruct_match eqn:modulo_zero in ceildiv_some.
+  - now apply div_zero in ceildiv_some.
+  - cbn in ceildiv_some.
+    destruct_match eqn:div_some in ceildiv_some;
+      try congruence.
+    now apply div_zero in div_some.
+Qed.
+Opaque ceildiv.
+Opaque ceildiv_.
+
+
+
+(* ---------------------------------------------------------------------- *)
+(* Set baker correct                                                      *)
+(* ---------------------------------------------------------------------- *)
+
+(* set_baker only changes freezeBaker in state *)
+Lemma set_baker_state_eq : forall prev_state new_state chain ctx new_acts param,
+  receive chain ctx prev_state (Some (FA2Token.other_msg (SetBaker param))) = Some (new_state, new_acts) ->
+    prev_state<| freezeBaker := param.(freezeBaker_) |> = new_state.
+Proof.
+  intros * receive_some.
+  receive_simpl.
+Qed.
+
+Lemma set_baker_freeze_baker_correct : forall prev_state new_state chain ctx new_acts param,
+  receive chain ctx prev_state (Some (FA2Token.other_msg (SetBaker param))) = Some (new_state, new_acts) ->
+    new_state.(freezeBaker) = param.(freezeBaker_).
+Proof.
+  intros * receive_some.
+  apply set_baker_state_eq in receive_some.
+  now subst.
+Qed.
+
+(* set_baker produces no new_acts *)
+Lemma set_baker_new_acts_correct : forall chain ctx prev_state param new_state new_acts,
+  receive chain ctx prev_state (Some (FA2Token.other_msg (SetBaker param))) = Some (new_state, new_acts) ->
+    new_acts = set_delegate_call param.(baker).
+Proof.
+  intros * receive_some.
+  receive_simpl.
+Qed.
+
+(* If the requirements are met then then receive on set_baker msg must succeed and
+    if receive on set_baker msg succeeds then requirements must hold *)
+Lemma set_baker_is_some : forall prev_state chain ctx param,
+  (ctx_amount ctx <= 0)%Z /\
+  prev_state.(selfIsUpdatingTokenPool) = false /\
+  ctx.(ctx_from) = prev_state.(manager) /\
+  prev_state.(freezeBaker) = false
+  <->
+  exists new_state new_acts, receive chain ctx prev_state (Some (FA2Token.other_msg (SetBaker param))) = Some (new_state, new_acts).
+Proof.
+  split.
+  - intros (amount_zero & not_updating & sender_is_manager & not_frozen).
+    do 2 eexists.
+    receive_simpl.
+    destruct_match eqn:updating_check.
+    destruct_match eqn:amount_check.
+    destruct_match eqn:sender_check.
+    destruct_match eqn:frozen_check.
+    + reflexivity.
+    + now rewrite not_frozen in frozen_check.
+    + now rewrite sender_is_manager, address_eq_refl in sender_check.
+    + receive_simpl.
+      now apply Z.ltb_ge in amount_zero.
+    + now rewrite not_updating in updating_check.
+  - intros (new_state & new_acts & receive_some).
+    receive_simpl.
+    rename H0 into ctx_amount_zero.
+    apply Z.ltb_ge in ctx_amount_zero.
+    repeat split; auto.
+    now destruct_address_eq.
+Qed.
+
+
+
+(* ---------------------------------------------------------------------- *)
+(* Set manager correct                                                    *)
+(* ---------------------------------------------------------------------- *)
+
+(* set_manager only changes manager in state *)
+Lemma set_manager_state_eq : forall prev_state new_state chain ctx new_acts new_manager,
+  receive chain ctx prev_state (Some (FA2Token.other_msg (SetManager new_manager))) = Some (new_state, new_acts) ->
+    prev_state<| manager := new_manager |> = new_state.
+Proof.
+  intros * receive_some.
+  receive_simpl.
+Qed.
+
+Lemma set_manager_manager_correct : forall prev_state new_state chain ctx new_acts new_manager,
+  receive chain ctx prev_state (Some (FA2Token.other_msg (SetManager new_manager))) = Some (new_state, new_acts) ->
+    new_state.(manager) = new_manager.
+Proof.
+  intros * receive_some.
+  apply set_manager_state_eq in receive_some.
+  now subst.
+Qed.
+
+(* set_manager produces no new_acts *)
+Lemma set_manager_new_acts_correct : forall chain ctx prev_state new_manager new_state new_acts,
+  receive chain ctx prev_state (Some (FA2Token.other_msg (SetManager new_manager))) = Some (new_state, new_acts) ->
+    new_acts = [].
+Proof.
+  intros * receive_some.
+  receive_simpl.
+Qed.
+
+(* If the requirements are met then then receive on set_manager msg must succeed and
+    if receive on set_manager msg succeeds then requirements must hold *)
+Lemma set_manager_is_some : forall prev_state chain ctx new_manager,
+  (ctx_amount ctx <= 0)%Z /\
+  prev_state.(selfIsUpdatingTokenPool) = false /\
+  ctx.(ctx_from) = prev_state.(manager)
+  <->
+  exists new_state new_acts, receive chain ctx prev_state (Some (FA2Token.other_msg (SetManager new_manager))) = Some (new_state, new_acts).
+Proof.
+  split.
+  - intros (amount_zero & not_updating & sender_is_manager).
+    do 2 eexists.
+    receive_simpl.
+    destruct_match eqn:updating_check.
+    destruct_match eqn:amount_check.
+    destruct_match eqn:sender_check.
+    + reflexivity.
+    + now rewrite sender_is_manager, address_eq_refl in sender_check.
+    + receive_simpl.
+      now apply Z.ltb_ge in amount_zero.
+    + now rewrite not_updating in updating_check.
+  - intros (new_state & new_acts & receive_some).
+    receive_simpl.
+    rename H0 into ctx_amount_zero.
+    apply Z.ltb_ge in ctx_amount_zero.
+    repeat split; auto.
+    now destruct_address_eq.
+Qed.
+
+
+(* ---------------------------------------------------------------------- *)
+(* Set liquidity address correct                                          *)
+(* ---------------------------------------------------------------------- *)
+
+(* set_lqt_address only changes lqt address in state *)
+Lemma set_lqt_address_state_eq : forall prev_state new_state chain ctx new_acts new_lqt_address,
+  receive chain ctx prev_state (Some (FA2Token.other_msg (SetLqtAddress new_lqt_address))) = Some (new_state, new_acts) ->
+    prev_state<| lqtAddress := new_lqt_address |> = new_state.
+Proof.
+  intros * receive_some.
+  receive_simpl.
+Qed.
+
+Lemma set_lqt_address_correct : forall prev_state new_state chain ctx new_acts new_lqt_address,
+  receive chain ctx prev_state (Some (FA2Token.other_msg (SetLqtAddress new_lqt_address))) = Some (new_state, new_acts) ->
+    new_state.(lqtAddress) = new_lqt_address.
+Proof.
+  intros * receive_some.
+  apply set_lqt_address_state_eq in receive_some.
+  now subst.
+Qed.
+
+(* set_lqt_address produces no new_acts *)
+Lemma set_lqt_address_new_acts_correct : forall chain ctx prev_state new_lqt_address new_state new_acts,
+  receive chain ctx prev_state (Some (FA2Token.other_msg (SetLqtAddress new_lqt_address))) = Some (new_state, new_acts) ->
+    new_acts = [].
+Proof.
+  intros * receive_some.
+  receive_simpl.
+Qed.
+
+(* If the requirements are met then then receive on set_lqt_address msg must succeed and
+    if receive on set_lqt_address msg succeeds then requirements must hold *)
+Lemma set_lqt_address_is_some : forall prev_state chain ctx new_lqt_address,
+  (ctx_amount ctx <= 0)%Z /\
+  prev_state.(selfIsUpdatingTokenPool) = false /\
+  ctx.(ctx_from) = prev_state.(manager) /\
+  prev_state.(lqtAddress) = prev_state.(nullAddress)
+  <->
+  exists new_state new_acts, receive chain ctx prev_state (Some (FA2Token.other_msg (SetLqtAddress new_lqt_address))) = Some (new_state, new_acts).
+Proof.
+  split.
+  - intros (amount_zero & not_updating & sender_is_manager & lqt_address_not_set).
+    do 2 eexists.
+    receive_simpl.
+    destruct_match eqn:updating_check.
+    destruct_match eqn:amount_check.
+    destruct_match eqn:sender_check.
+    destruct_match eqn:lqt_check.
+    + reflexivity.
+    + now rewrite lqt_address_not_set, address_eq_refl in lqt_check.
+    + now rewrite sender_is_manager, address_eq_refl in sender_check.
+    + receive_simpl.
+      now apply Z.ltb_ge in amount_zero.
+    + now rewrite not_updating in updating_check.
+  - intros (new_state & new_acts & receive_some).
+    receive_simpl.
+    rename H0 into ctx_amount_zero.
+    rename H2 into lqt_address_not_set.
+    apply Z.ltb_ge in ctx_amount_zero.
+    repeat split; auto;
+      now destruct_address_eq.
+Qed.
+
+(* ---------------------------------------------------------------------- *)
+(* default entrypoint correct                                             *)
+(* ---------------------------------------------------------------------- *)
+
+(* default_ only changes xtzPool in state *)
+Lemma default_state_eq : forall prev_state new_state chain ctx new_acts,
+  receive chain ctx prev_state None = Some (new_state, new_acts) ->
+    prev_state<| xtzPool := prev_state.(xtzPool) + Z.to_N (ctx.(ctx_amount)) |> = new_state.
+Proof.
+  intros * receive_some.
+  receive_simpl.
+Qed.
+
+Lemma default_correct : forall prev_state new_state chain ctx new_acts,
+  receive chain ctx prev_state None = Some (new_state, new_acts) ->
+    new_state.(xtzPool) = prev_state.(xtzPool) + Z.to_N (ctx.(ctx_amount)).
+Proof.
+  intros * receive_some.
+  apply default_state_eq in receive_some.
+  now subst.
+Qed.
+
+(* default_ produces no new_acts *)
+Lemma default_new_acts_correct : forall chain ctx prev_state new_state new_acts,
+  receive chain ctx prev_state None = Some (new_state, new_acts) ->
+    new_acts = [].
+Proof.
+  intros * receive_some.
+  receive_simpl.
+Qed.
+
+(* If the requirements are met then then receive on None msg must succeed and
+    if receive on None msg succeeds then requirements must hold *)
+Lemma default_entrypoint_is_some : forall prev_state chain ctx,
+  prev_state.(selfIsUpdatingTokenPool) = false
+  <->
+  exists new_state new_acts, receive chain ctx prev_state None = Some (new_state, new_acts).
+Proof.
+  split.
+  - intros not_updating.
+    do 2 eexists.
+    receive_simpl.
+    destruct_match eqn:updating_check.
+    + reflexivity.
+    + now rewrite not_updating in updating_check.
+  - intros (new_state & new_acts & receive_some).
+    receive_simpl.
+Qed.
+
+(* ---------------------------------------------------------------------- *)
+(* update token pool correct                                              *)
+(* ---------------------------------------------------------------------- *)
+
+(* update_token_pool only changes selfIsUpdatingTokenPool in state *)
+Lemma update_token_pool_state_eq : forall prev_state new_state chain ctx new_acts,
+  receive chain ctx prev_state (Some (FA2Token.other_msg UpdateTokenPool)) = Some (new_state, new_acts) ->
+    prev_state<| selfIsUpdatingTokenPool := true |> = new_state.
+Proof.
+  intros * receive_some.
+  receive_simpl.
+Qed.
+
+Lemma update_token_pool_correct : forall prev_state new_state chain ctx new_acts,
+  receive chain ctx prev_state (Some (FA2Token.other_msg UpdateTokenPool)) = Some (new_state, new_acts) ->
+    new_state.(selfIsUpdatingTokenPool) = true.
+Proof.
+  intros * receive_some.
+  apply update_token_pool_state_eq in receive_some.
+  now subst.
+Qed.
+
+(* update_token_pool produces an call act with amount = 0, calling
+    the token contract with a balance of request *)
+Lemma update_token_pool_new_acts_correct : forall chain ctx prev_state new_state new_acts,
+  receive chain ctx prev_state (Some (FA2Token.other_msg UpdateTokenPool)) = Some (new_state, new_acts) ->
+    new_acts = [
+      act_call prev_state.(tokenAddress) 0%Z (serialize
+        (msg_balance_of (Build_balance_of_param 
+          ([Build_balance_of_request ctx.(ctx_contract_address) prev_state.(tokenId)])
+          (FA2Interface.Build_callback _ None))))
+    ].
+Proof.
+  intros * receive_some.
+  receive_simpl.
+Qed.
+
+(* If the requirements are met then then receive on update_token_pool msg must succeed and
+    if receive on update_token_pool msg succeeds then requirements must hold *)
+Lemma update_token_pool_is_some : forall prev_state chain ctx,
+  (ctx_amount ctx <= 0)%Z /\
+  prev_state.(selfIsUpdatingTokenPool) = false /\
+  address_is_contract ctx.(ctx_from) = false
+  <->
+  exists new_state new_acts, receive chain ctx prev_state (Some (FA2Token.other_msg UpdateTokenPool)) = Some (new_state, new_acts).
+Proof.
+  split.
+  - intros (amount_zero & not_updating & sender_not_contract).
+    do 2 eexists.
+    receive_simpl.
+    destruct_match eqn:sender_check.
+    destruct_match eqn:amount_check.
+    destruct_match eqn:updating_check.
+    + reflexivity.
+    + now rewrite not_updating in updating_check.
+    + receive_simpl.
+      now apply Z.ltb_ge in amount_zero.
+    + now rewrite sender_not_contract in sender_check.
+  - intros (new_state & new_acts & receive_some).
+    receive_simpl.
+    rename H0 into ctx_amount_zero.
+    now apply Z.ltb_ge in ctx_amount_zero.
+Qed.
+
+(* ---------------------------------------------------------------------- *)
+(* update token pool internal correct                                     *)
+(* ---------------------------------------------------------------------- *)
+
+(* update_token_pool_internal only changes selfIsUpdatingTokenPool and tokenPool in state *)
+Lemma update_token_pool_internal_state_eq : forall prev_state new_state chain ctx new_acts responses,
+  receive chain ctx prev_state (Some (FA2Token.receive_balance_of_param responses)) = Some (new_state, new_acts) ->
+    prev_state<| selfIsUpdatingTokenPool := false |>
+              <| tokenPool := match responses with 
+                              | [] => 0
+                              | response :: t => response.(balance)
+                              end |> = new_state.
+Proof.
+  intros * receive_some.
+  receive_simpl.
+  rename H1 into response.
+  destruct_match eqn:resonses_empty_check in response;
+    try congruence.
+  now inversion_clear response.
+Qed.
+
+Lemma update_token_pool_internal_update_correct : forall prev_state new_state chain ctx new_acts responses,
+  receive chain ctx prev_state (Some (FA2Token.receive_balance_of_param responses)) = Some (new_state, new_acts) ->
+    new_state.(selfIsUpdatingTokenPool) = false.
+Proof.
+  intros * receive_some.
+  apply update_token_pool_internal_state_eq in receive_some.
+  now subst.
+Qed.
+
+(* update_token_pool_internal produces no new actions *)
+Lemma update_token_pool_internal_new_acts_correct : forall chain ctx prev_state new_state new_acts responses,
+  receive chain ctx prev_state (Some (FA2Token.receive_balance_of_param responses)) = Some (new_state, new_acts) ->
+    new_acts = [].
+Proof.
+  intros * receive_some.
+  receive_simpl.
+Qed.
+
+(* If the requirements are met then then receive on update_token_pool_internal msg must succeed and
+    if receive on update_token_pool_internal msg succeeds then requirements must hold *)
+Lemma update_token_pool_internal_is_some : forall prev_state chain ctx responses,
+  (ctx_amount ctx <= 0)%Z /\
+  prev_state.(selfIsUpdatingTokenPool) = true /\
+  ctx.(ctx_from) = prev_state.(tokenAddress) /\
+  responses <> []
+  <->
+  exists new_state new_acts, receive chain ctx prev_state (Some (FA2Token.receive_balance_of_param responses)) = Some (new_state, new_acts).
+Proof.
+  split.
+  - intros (amount_zero & updating & sender_is_token_contract & responses_not_empty).
+    unfold receive. cbn.
+    destruct_match eqn:sender_check.
+    destruct_match eqn:amount_check.
+    destruct_match eqn:response.
+    destruct_match eqn:response_check in response.
+    + congruence.
+    + eauto.
+    + now destruct_match in response.
+    + receive_simpl.
+      now apply Z.ltb_ge in amount_zero.
+    + now rewrite updating, sender_is_token_contract, address_eq_refl in sender_check.
+  - intros (new_state & new_acts & receive_some).
+    receive_simpl.
+    rename H0 into ctx_amount_zero.
+    rename H into sender_check.
+    rename H1 into responses_check.
+    apply Bool.orb_false_elim in sender_check as
+      (is_updating & sender_is_token_contract).
+    apply Z.ltb_ge in ctx_amount_zero.
+    destruct responses eqn:response in responses_check;
+      try congruence.
+    subst.
+    repeat split; auto.
+    + now apply Bool.negb_false_iff in is_updating.
+    + now destruct_address_eq.
+Qed.
+
+(* ---------------------------------------------------------------------- *)
+(* Add liquidity correct                                                  *)
+(* ---------------------------------------------------------------------- *)
+
+(* add_liquidity only changes selfIsUpdatingTokenPool and tokenPool in state *)
+Lemma add_liquidity_state_eq : forall prev_state new_state chain ctx new_acts param,
+  let lqt_minted := Z.to_N ctx.(ctx_amount) * prev_state.(lqtTotal) / prev_state.(xtzPool) in
+  let tokens_deposited := ceildiv_ (Z.to_N ctx.(ctx_amount) * prev_state.(tokenPool)) prev_state.(xtzPool) in
+  receive chain ctx prev_state (Some (FA2Token.other_msg (AddLiquidity param))) = Some (new_state, new_acts) ->
+    prev_state<| lqtTotal := prev_state.(lqtTotal) +  lqt_minted |>
+              <| tokenPool := prev_state.(tokenPool) + tokens_deposited |>
+              <| xtzPool := prev_state.(xtzPool) + Z.to_N ctx.(ctx_amount) |> = new_state.
+Proof.
+  intros * receive_some.
+  receive_simpl.
+  rename H1 into div_some.
+  rename H2 into ceildiv_some.
+  apply div_eq in div_some as (? & _).
+  apply ceildiv_eq in ceildiv_some as (? & _).
+  now subst.
+Qed.
+
+Lemma add_liquidity_correct : forall prev_state new_state chain ctx new_acts param,
+  receive chain ctx prev_state (Some (FA2Token.other_msg (AddLiquidity param))) = Some (new_state, new_acts) ->
+    new_state.(lqtTotal) = prev_state.(lqtTotal) + Z.to_N ctx.(ctx_amount) * prev_state.(lqtTotal) / prev_state.(xtzPool) /\
+    new_state.(tokenPool) = prev_state.(tokenPool) + ceildiv_ (Z.to_N ctx.(ctx_amount) * prev_state.(tokenPool)) prev_state.(xtzPool) /\
+    new_state.(xtzPool) = prev_state.(xtzPool) + Z.to_N ctx.(ctx_amount).
+Proof.
+  intros * receive_some.
+  apply add_liquidity_state_eq in receive_some.
+  now subst.
+Qed.
+
+(* add_liquidity should two acts
+    1: an call action to the token contract requesting <tokens_deposited> tokens to be moved from <owner> to this contract
+    2: an call action to the lqt contract requsting <lqt_minted> tokens to be minted to <owner>
+ *)
+Lemma add_liquidity_new_acts_correct : forall chain ctx prev_state new_state new_acts param,
+  let lqt_minted := Z.to_N ctx.(ctx_amount) * prev_state.(lqtTotal) / prev_state.(xtzPool) in
+  let tokens_deposited := ceildiv_ (Z.to_N ctx.(ctx_amount) * prev_state.(tokenPool)) prev_state.(xtzPool) in
+  receive chain ctx prev_state (Some (FA2Token.other_msg (AddLiquidity param))) = Some (new_state, new_acts) ->
+    new_acts =
+    [
+      (act_call prev_state.(tokenAddress) 0%Z
+        (serialize (FA2Token.msg_transfer
+        [build_transfer param.(owner) ctx.(ctx_contract_address) prev_state.(tokenId) tokens_deposited None])));
+      (act_call prev_state.(lqtAddress) 0%Z
+        (serialize (Dexter2FA12.msg_mint_or_burn {| target := param.(owner); quantity := Z.of_N lqt_minted|})))
+    ].
+Proof.
+  intros * receive_some.
+  receive_simpl.
+  rename H1 into div_some.
+  rename H2 into ceildiv_some.
+  apply div_eq in div_some as (? & _).
+  apply ceildiv_eq in ceildiv_some as (? & _).
+  subst.
+  unfold token_transfer.
+  repeat f_equal.
+  give_up.
+Abort.
+
+(* In the informal specification it is stated that tokens should be trasnfered from owner,
+    but in the implementation it is trasnfered from the sender.
+   For this we assume that the implementation is correct over the informal specification since
+    that is what other formalizations seem to have assumed *)
+Lemma add_liquidity_new_acts_correct : forall chain ctx prev_state new_state new_acts param,
+  let lqt_minted := Z.to_N ctx.(ctx_amount) * prev_state.(lqtTotal) / prev_state.(xtzPool) in
+  let tokens_deposited := ceildiv_ (Z.to_N ctx.(ctx_amount) * prev_state.(tokenPool)) prev_state.(xtzPool) in
+  receive chain ctx prev_state (Some (FA2Token.other_msg (AddLiquidity param))) = Some (new_state, new_acts) ->
+    new_acts =
+    [
+      (act_call prev_state.(tokenAddress) 0%Z
+        (serialize (FA2Token.msg_transfer
+        [build_transfer ctx.(ctx_from) ctx.(ctx_contract_address) prev_state.(tokenId) tokens_deposited None])));
+      (act_call prev_state.(lqtAddress) 0%Z
+        (serialize (Dexter2FA12.msg_mint_or_burn {| target := param.(owner); quantity := Z.of_N lqt_minted|})))
+    ].
+Proof.
+  intros * receive_some.
+  receive_simpl.
+  rename H1 into div_some.
+  rename H2 into ceildiv_some.
+  apply div_eq in div_some as (? & _).
+  apply ceildiv_eq in ceildiv_some as (? & _).
+  now subst.
+Qed.
+
+(* If the requirements are met then then receive on add_liquidity msg must succeed and
+    if receive on add_liquidity msg succeeds then requirements must hold *)
+Lemma add_liquidity_is_some : forall prev_state chain ctx param,
+  let lqt_minted := Z.to_N ctx.(ctx_amount) * prev_state.(lqtTotal) / prev_state.(xtzPool) in
+  let tokens_deposited := ceildiv_ (Z.to_N ctx.(ctx_amount) * prev_state.(tokenPool)) prev_state.(xtzPool) in
+  prev_state.(selfIsUpdatingTokenPool) = false /\
+  (current_slot chain < param.(add_deadline))%nat /\
+  tokens_deposited <= param.(maxTokensDeposited)  /\
+  param.(minLqtMinted) <= lqt_minted /\
+  prev_state.(xtzPool) <> 0 /\
+  prev_state.(lqtAddress) <> prev_state.(nullAddress)
+  <->
+  exists new_state new_acts, receive chain ctx prev_state (Some (FA2Token.other_msg (AddLiquidity param))) = Some (new_state, new_acts).
+Proof.
+  split.
+  - intros (not_updating & deadline_not_hit & max_tokens_not_hit &
+            enough_minted & xtzPool_not_zero & lqt_addr_set).
+    unfold receive.
+    cbn.
+    destruct_match eqn:updating_check.
+    destruct_match eqn:deadline_check.
+    destruct_match eqn:div_check.
+    destruct_match eqn:ceildiv_check.
+    destruct_match eqn:max_tokens_check.
+    destruct_match eqn:min_lqt_check.
+    destruct_match eqn:mint_act; try congruence;
+    destruct_match eqn:lqt_addr_set_check in mint_act; try congruence.
+    + inversion_clear div_check.
+      inversion_clear ceildiv_check.
+      eauto.
+    + apply address_eq_ne in lqt_addr_set.
+      now rewrite lqt_addr_set in lqt_addr_set_check.
+    + apply div_eq in div_check as [<- _].
+      apply N.ltb_ge in enough_minted.
+      now rewrite enough_minted in min_lqt_check.
+    + apply ceildiv_eq in ceildiv_check as [<- _].
+      apply N.ltb_ge in max_tokens_not_hit.
+      now rewrite max_tokens_not_hit in max_tokens_check.
+    + now apply ceildiv_zero in ceildiv_check.
+    + now apply div_zero in div_check.
+    + apply leb_correct_conv in deadline_not_hit.
+      now rewrite deadline_not_hit in deadline_check.
+    + now rewrite not_updating in updating_check.
+  - intros (new_state & new_acts & receive_some).
+    receive_simpl.
+    rename H1 into div_some.
+    rename H2 into ceildiv_some.
+    rename H0 into deadline_not_hit.
+    rename H3 into max_not_hit.
+    rename H4 into min_not_hit.
+    apply div_eq in div_some as [<- xtzPool_zero].
+    apply ceildiv_eq in ceildiv_some as [<- _].
+    apply leb_complete_conv in deadline_not_hit.
+    apply N.ltb_ge in max_not_hit.
+    apply N.ltb_ge in min_not_hit.
+    repeat split; auto.
+    now destruct_address_eq.
+Qed.
+
+(* ---------------------------------------------------------------------- *)
+(* Remove liquidity correct                                               *)
+(* ---------------------------------------------------------------------- *)
+
+(*
+TODO
+
+  general
+    freezebaker = true -> cannot be changed
+    constants are constant
+    only set_manager can change manager
+    lqt address set -> cannot be changed
+    updating = true -> all msg's other that update_token_pool_internal will fail
+    
+    if msg <> remove_lqt then worth of contract must not decrease
+    after update token balance will be in sync
+    if no token transfers happen then token balance will always be in sync
+    xtzPool always equals contract balance if deploy amount = 0
+    lqt token pool always equal actual total supply
+    all transfer produced are valid
+*)
+
+(* ---------------------------------------------------------------------- *)
+(* xtz to token correct                                                   *)
+(* ---------------------------------------------------------------------- *)
+
+(* ---------------------------------------------------------------------- *)
+(* token to xtz correct                                                   *)
+(* ---------------------------------------------------------------------- *)
+
+(* ---------------------------------------------------------------------- *)
+(* token to token correct                                                 *)
+(* ---------------------------------------------------------------------- *)
+
+
+
+
+
 End Theories.
 End Dexter.
